run_default, start of run_code

CoqOfRust/alloc/vec/links/mod.v
@@ -41,3 +41,16 @@ Module Impl_Clone_for_Vec.
     }
   Defined.
 End Impl_Clone_for_Vec.
+
+Module Impl_Default_for_Vec.
+  Definition run_default {T A : Set} `{Link T} `{Link A} : default.Default.Run_default (Vec.t T A).
+  Admitted.
+
+  Definition run {T A : Set} `{Link T} `{Link A} : default.Default.Run (Vec.t T A).
+  Proof.
+    constructor.
+    { (* clone *)
+      exact run_default.
+    }
+  Defined.
+End Impl_Default_for_Vec.
