CoqOfRust/core/slice/links/mod.v
@@ -1,0 +1,17 @@
+Require Import CoqOfRust.CoqOfRust.
+Require Import links.M.
+Require Import core.slice.mod.
+Import Run.
+
+Module Impl_Slice.
+  Definition Self (T : Set) `{Link T} : Set := list T.
+  
+  (*
+    pub fn get<I>(&self, index: I) -> Option<&I::Output>
+    where
+        I: SliceIndex<Self>,
+    {
+        index.get(self)
+    }
+  *)
+End Impl_Slice.
